lakefile.lean
@@ -6,34 +6,34 @@ package «hex-berlekamp-zassenhaus» where
   leanOptions := #[⟨`doc.verso, true⟩, ⟨`doc.verso.suggestions, false⟩]
 
 require HexBerlekamp from git
-  "https://github.com/leanprover/hex-berlekamp.git" @ "v0.5.0"
+  "https://github.com/leanprover/hex-berlekamp.git" @ "v0.6.0"
 
 require HexHensel from git
-  "https://github.com/leanprover/hex-hensel.git" @ "v0.5.0"
+  "https://github.com/leanprover/hex-hensel.git" @ "v0.6.0"
 
 require HexLLL from git
-  "https://github.com/leanprover/hex-lll.git" @ "v0.5.0"
+  "https://github.com/leanprover/hex-lll.git" @ "v0.6.0"
 
 require HexBasic from git
-  "https://github.com/leanprover/hex-basic.git" @ "v0.5.0"
+  "https://github.com/leanprover/hex-basic.git" @ "v0.6.0"
 
 require HexArith from git
-  "https://github.com/leanprover/hex-arith.git" @ "v0.5.0"
+  "https://github.com/leanprover/hex-arith.git" @ "v0.6.0"
 
 require HexPrimality from git
-  "https://github.com/leanprover/hex-primality.git" @ "v0.5.0"
+  "https://github.com/leanprover/hex-primality.git" @ "v0.6.0"
 
 require HexPoly from git
-  "https://github.com/leanprover/hex-poly.git" @ "v0.5.0"
+  "https://github.com/leanprover/hex-poly.git" @ "v0.6.0"
 
 require HexMatrix from git
-  "https://github.com/leanprover/hex-matrix.git" @ "v0.5.0"
+  "https://github.com/leanprover/hex-matrix.git" @ "v0.6.0"
 
 require HexModArith from git
-  "https://github.com/leanprover/hex-mod-arith.git" @ "v0.5.0"
+  "https://github.com/leanprover/hex-mod-arith.git" @ "v0.6.0"
 
 require HexPolyZ from git
-  "https://github.com/leanprover/hex-poly-z.git" @ "v0.5.0"
+  "https://github.com/leanprover/hex-poly-z.git" @ "v0.6.0"
 
 @[default_target]
 lean_lib HexBerlekampZassenhaus
